src/Init/Data/Range/New/Iteration.lean
@@ -7,97 +7,32 @@ open Std.Iterators
 
 @[always_inline, inline]
 def PRange.iterInternal [UpwardEnumerable α] [HasRange shape α] [UpwardEnumerableRange shape α]
-    (r : PRange shape α) :=
-  (⟨⟨UpwardEnumerableRange.init r.lower, r.upper⟩⟩ : Iter (α := Types.RangeIterator shape α) α)
+    (r : PRange shape α) : Iter (α := Types.RangeIterator shape α) α :=
+  ⟨⟨UpwardEnumerableRange.init r.lower, r.upper⟩⟩
 
 @[always_inline, inline]
-def PRange.iter [RangeIter shape α] (r : PRange shape α) :=
-  (RangeIter.iter r : Iter α)
+def PRange.iter [UpwardEnumerable α] [HasRange shape α] [UpwardEnumerableRange shape α]
+    (r : PRange shape α) : Iter (α := Types.RangeIterator shape α) α :=
+  PRange.iterInternal r
 
 @[always_inline, inline]
-def PRange.size [RangeIter shape α] (r : PRange shape α)
-    [Iterator (RangeIter.State r) Id α] [IteratorSize (RangeIter.State r) Id] :
-    Nat :=
+def PRange.size [UpwardEnumerable α] [HasRange shape α] [UpwardEnumerableRange shape α]
+    (r : PRange shape α) [IteratorSize (Types.RangeIterator shape α) Id] : Nat :=
   r.iter.size
 
 @[always_inline, inline]
-def PRange.toList [RangeIter shape α] (r : PRange shape α)
-    [Iterator (RangeIter.State r) Id α] [Finite (RangeIter.State r) Id]
-    [IteratorCollect (RangeIter.State r) Id Id] :
-    List α :=
+def PRange.toList [UpwardEnumerable α] [HasRange shape α] [UpwardEnumerableRange shape α]
+    (r : PRange shape α)
+    [Iterator (Types.RangeIterator shape α) Id α] [Finite (Types.RangeIterator shape α) Id]
+    [IteratorCollect (Types.RangeIterator shape α) Id Id] : List α :=
   r.iterInternal.toList
 
-instance [i : RangeIter shape α] [∀ r, ForIn m (Iter (α := i.State r) α) α] :
-    ForIn m (PRange shape α) α where
-  forIn r := forIn r.iter
+-- instance [UpwardEnumerable α] [HasRange shape α] [UpwardEnumerableRange shape α]
+--     [ForIn' m (Iter (α := Types.RangeIterator shape α) α) α inferInstance] :
+--     ForIn' m (PRange shape α) α where
+--   forIn r := forIn r.iter
 
 section Iterator
-
-@[always_inline, inline]
-def Range.succIterator [Succ? α] (init : Option α) (Predicate : α → Bool) :
-    (Iter (α := Types.RangeIterator α inferInstance Predicate) α) :=
-  ⟨⟨init⟩⟩
-
--- @[always_inline, inline]
--- def Range.SuccIterator.next [Succ? α] (stepSize : Nat) (Predicate : α → Bool)
---     {h : stepSize > 0} (it : SuccIterator stepSize Predicate h) : α :=
---   it.inner.internalState.next
-
--- @[no_expose]
--- instance [Succ? α] (stepSize : Nat) (Predicate : α → Bool) (h) :
---     Iterator (Range.SuccIterator stepSize Predicate h) Id α := by
---   unfold Range.SuccIterator
---   infer_instance
-
--- @[no_expose]
--- instance [Monad m] [Succ? α] (stepSize : Nat) (Predicate : α → Bool) (h) :
---     IteratorCollect (Range.SuccIterator stepSize Predicate h) Id m := by
---   unfold Range.SuccIterator
---   infer_instance
-
--- @[no_expose]
--- instance [Monad m] [Succ? α] (stepSize : Nat) (Predicate : α → Bool) (h) :
---     IteratorCollectPartial (Range.SuccIterator stepSize Predicate h) Id m := by
---   unfold Range.SuccIterator
---   infer_instance
-
--- @[no_expose]
--- instance [Monad m] [MonadLiftT Id m] [Succ? α] (stepSize : Nat) (Predicate : α → Bool) (h) :
---     IteratorLoop (Range.SuccIterator stepSize Predicate h) Id m := by
---   unfold Range.SuccIterator
---   infer_instance
-
--- @[no_expose]
--- instance [Monad m] [MonadLiftT Id m] [Succ? α] (stepSize : Nat) (Predicate : α → Bool) (h) :
---     IteratorLoopPartial (Range.SuccIterator stepSize Predicate h) Id m := by
---   unfold Range.SuccIterator
---   infer_instance
-
--- TODO: Should we hide the ≤ or < predicates behind some identifier to avoid accidental rewriting?
-@[expose]
-instance [Succ? α] [LE α] [DecidableLE α] : RangeIter ⟨.closed, .closed⟩ α :=
-  .of fun r => Range.succIterator (some r.lower) (fun a => a ≤ r.upper)
-
-instance [Succ? α] [LT α] [DecidableLT α] : RangeIter ⟨.closed, .open⟩ α :=
-  .of fun r => Range.succIterator (some r.lower) (fun a => a < r.upper)
-
-instance [Succ? α] [LT α] [DecidableLT α] : RangeIter ⟨.closed, .unbounded⟩ α :=
-  .of fun r => Range.succIterator (some r.lower) (fun _ => True)
-
-instance [Succ? α] [LE α] [DecidableLE α] : RangeIter ⟨.open, .closed⟩ α :=
-  .of fun r => Range.succIterator (Succ?.succ? r.lower) (fun a => a ≤ r.upper)
-
-instance [Succ? α] [LT α] [DecidableLT α] : RangeIter ⟨.open, .open⟩ α :=
-  .of fun r => Range.succIterator (Succ?.succ? r.lower) (fun a => a < r.upper)
-
-instance [Succ? α] [LT α] [DecidableLT α] : RangeIter ⟨.open, .unbounded⟩ α :=
-  .of fun r => Range.succIterator (Succ?.succ? r.lower) (fun _ => True)
-
-instance [Succ? α] [LE α] [DecidableLE α] [HasDownwardUnboundedRanges α] :
-    RangeIter ⟨.unbounded, .closed⟩ α :=
-  .of fun r => Range.succIterator (some HasDownwardUnboundedRanges.min) (· ≤ r.upper)
-
--- TODO: iterators for ranges that are unbounded downwards
 
 -- theorem Range.SuccIterator.succ?_eq_some_of_isPlausibleSuccessorOf [Succ? α] [LE α] [DecidableLE α]
 --     {it' it : Iter (α := Types.RangeIterator α inferInstance P) α}
@@ -108,66 +43,117 @@ instance [Succ? α] [LE α] [DecidableLE α] [HasDownwardUnboundedRanges α] :
 --     TakeWhile.isPlausibleSuccessorOf_inner_of_isPlausibleSuccessorOf |>
 --     RepeatIterator.Monadic.next_eq_some_of_isPlausibleSuccessorOf
 
-@[no_expose]
-instance [Succ? α] [LE α] [DecidableLE α] [LawfulLESucc? α] [Monad m]
-    [∀ a, Finite (Types.RangeIterator α inferInstance (· ≤ a)) Id] :
-    ForIn' m (PRange ⟨.closed, .closed⟩ α) α inferInstance where
+private theorem RangeIterator.isPlausibleIndirectOutput_iff.aux
+    [UpwardEnumerable α] [HasRange shape α] [UpwardEnumerableRange shape α]
+    [LawfulUpwardEnumerable α] [LawfulUpwardEnumerableRange shape α]
+    {r : PRange shape α} {it : Iter (α := Types.RangeIterator shape α) α} {a : α}
+    (h : ∃ next, it.internalState.next = some next ∧ HasRange.SatisfiesLowerBound r.lower next)
+    (h' : it.IsPlausibleIndirectOutput a)
+    (hu : it.internalState.upperBound = r.upper) :
+    a ∈ r := by
+  induction h'
+  case direct it out h' =>
+    simp only [Types.RangeIterator.isPlausibleOutput_iff, hu] at h'
+    obtain ⟨next, hn, hl⟩ := h
+    simp only [h'.1, Option.some.injEq] at hn
+    cases hn
+    exact ⟨hl, h'.2⟩
+  case indirect it it' out  hs ho ih =>
+    rw [Types.RangeIterator.isPlausibleSuccessorOf_iff] at hs
+    obtain ⟨next, hn, h₁, h₂, hs⟩ := hs
+    apply ih
+    · rw [← hs] at hu
+      have ho' := Types.RangeIterator.isSome_next_of_isPlausibleIndirectOutput ho
+      rw [Option.isSome_iff_exists] at ho'
+      obtain ⟨a, ha⟩ := ho'
+      rw [ha] at h₂
+      refine ⟨a, ha, ?_⟩
+      apply LawfulUpwardEnumerableRange.satisfiesLowerBound_of_le r.lower next a
+      · obtain ⟨_, hn', hl⟩ := h
+        simp only [hn] at hn'
+        cases hn'
+        exact hl
+      · refine ⟨1, ?_⟩
+        simp [LawfulUpwardEnumerable.succMany?_succ, LawfulUpwardEnumerable.succMany?_zero, h₂]
+    · simp [*]
+
+theorem RangeIterator.isPlausibleIndirectOutput_iff'
+    [UpwardEnumerable α] [HasRange shape α] [UpwardEnumerableRange shape α]
+    [LawfulUpwardEnumerable α] [LawfulUpwardEnumerableRange shape α]
+    {it : Iter (α := Types.RangeIterator shape α) α} {out : α} :
+    it.IsPlausibleIndirectOutput out ↔
+      ∃ n, it.internalState.next.bind (UpwardEnumerable.succMany? n ·) = some out ∧
+        HasRange.SatisfiesUpperBound it.internalState.upperBound out := by
+  constructor
+  · intro h
+    induction h
+    case direct h =>
+      rw [Types.RangeIterator.isPlausibleOutput_iff] at h
+      refine ⟨0, by simp [h, LawfulUpwardEnumerable.succMany?_zero]⟩
+    case indirect h _ ih =>
+      rw [Types.RangeIterator.isPlausibleSuccessorOf_iff] at h
+      obtain ⟨n, hn⟩ := ih
+      obtain ⟨a, ha, h₁, h₂, h₃⟩ := h
+      refine ⟨n + 1, ?_⟩
+      simp [ha, ← h₃, hn.2, LawfulUpwardEnumerable.succMany?_succ_eq_succ_bind_succMany, h₂, hn]
+  · rintro ⟨n, hn, hu⟩
+    induction n generalizing it
+    case zero =>
+      apply Iter.IsPlausibleIndirectOutput.direct
+      rw [Types.RangeIterator.isPlausibleOutput_iff]
+      exact ⟨by simpa [LawfulUpwardEnumerable.succMany?_zero] using hn, hu⟩
+    case succ ih =>
+      cases hn' : it.internalState.next
+      · simp [hn'] at hn
+      rename_i a
+      simp [hn'] at hn
+      have hle : UpwardEnumerable.le a out := ⟨_, hn⟩
+      rw [LawfulUpwardEnumerable.succMany?_succ_eq_succ_bind_succMany] at hn
+      cases hn' : UpwardEnumerable.succ? a
+      · simp [hn'] at hn
+      rename_i a'
+      simp [hn'] at hn
+      specialize ih (it := ⟨some a', it.internalState.upperBound⟩) hn hu
+      refine Iter.IsPlausibleIndirectOutput.indirect ?_ ih
+      rw [Types.RangeIterator.isPlausibleSuccessorOf_iff]
+      refine ⟨a, ‹_›, ?_, hn', rfl⟩
+      apply LawfulUpwardEnumerableRange.satisfiesUpperBound_of_le _ a out
+      · exact hu
+      · exact hle
+
+theorem RangeIterator.isPlausibleIndirectOutput_iff
+    [UpwardEnumerable α] [HasRange shape α] [UpwardEnumerableRange shape α]
+    [LawfulUpwardEnumerable α] [LawfulUpwardEnumerableRange shape α]
+    {r : PRange shape α} {a : α} :
+    r.iterInternal.IsPlausibleIndirectOutput a ↔ a ∈ r := by
+  rw [isPlausibleIndirectOutput_iff']
+  constructor
+  · rintro ⟨n, hn, hu⟩
+    refine ⟨?_, hu⟩
+    rw [LawfulUpwardEnumerableRange.satisfiesLowerBound_iff]
+    cases hr : r.iterInternal.internalState.next
+    · simp [hr] at hn
+    rw [hr, Option.bind_some] at hn
+    exact ⟨_, hr, n, hn⟩
+  · rintro ⟨hl, hu⟩
+    rw [LawfulUpwardEnumerableRange.satisfiesLowerBound_iff] at hl
+    obtain ⟨_, hr, n, hn⟩ := hl
+    exact ⟨n, by simp [PRange.iterInternal, hr, hn], hu⟩
+
+instance [UpwardEnumerable α] [HasRange shape α] [UpwardEnumerableRange shape α]
+    [LawfulUpwardEnumerable α] [LawfulUpwardEnumerableRange shape α]
+    [Monad m] [Finite (Types.RangeIterator shape α) Id] :
+    ForIn' m (PRange shape α) α inferInstance where
   forIn' r init f := by
     haveI : MonadLift Id m := ⟨Std.Internal.idToMonad (α := _)⟩
-    refine ForIn'.forIn' (α := α) r.iter init (fun a ha acc => f a ?_ acc)
-    sorry
-    -- have hle : r.lower ≤ r.iter.internalState.next := by exact LawfulLESucc?.le_rfl (α := α)
-    -- generalize r.iter = it at ha hle
-    -- induction ha with
-    -- | direct =>
-    --   rename_i it out h
-    --   rcases h with ⟨it', h, h'⟩
-    --   refine ⟨?_, ?_⟩
-    --   · rcases h with ⟨rfl, _⟩
-    --     exact hle
-    --   · simpa [← PostconditionT.pure_eq_pure] using h'
-    -- | indirect =>
-    --   rename_i it it' it'' out h h' ih
-    --   apply ih
-    --   replace h := Range.SuccIterator.succ?_eq_some_of_isPlausibleSuccessorOf h
-    --   exact LawfulLESucc?.le_succAtIdx?_of_le (α := α) hle h
-
-@[no_expose]
-instance [Succ? α] [LT α] [DecidableLT α] [LE α] [DecidableLE α] [LawfulLESucc? α] [Monad m]
-    [∀ a, Finite (Types.RangeIterator α inferInstance (· < a)) Id] :
-    ForIn' m (PRange ⟨.closed, .open⟩ α) α inferInstance where
-  forIn' r init f := by
-    haveI : MonadLift Id m := ⟨Std.Internal.idToMonad (α := _)⟩
-    refine ForIn'.forIn' (α := α) r.iter init (fun a ha acc => f a ?_ acc)
-    sorry
-    -- have hle : r.lower ≤ r.iter.internalState.next := by exact LawfulLESucc?.le_rfl (α := α)
-    -- generalize r.iter = it at ha hle
-    -- induction ha with
-    -- | direct =>
-    --   rename_i it out h
-    --   rcases h with ⟨it', h, h'⟩
-    --   refine ⟨?_, ?_⟩
-    --   · rcases h with ⟨rfl, _⟩
-    --     exact hle
-    --   · simpa [← PostconditionT.pure_eq_pure] using h'
-    -- | indirect =>
-    --   rename_i it it' it'' out h h' ih
-    --   apply ih
-    --   replace h := Range.SuccIterator.succ?_eq_some_of_isPlausibleSuccessorOf h
-    --   exact LawfulLESucc?.le_succAtIdx?_of_le (α := α) hle h
-
--- instance [Succ? α] [LE α] [DecidableLE α] [LawfulLESucc? α]
---     [HasDownwardUnboundedRanges α] [Monad m]
---     [∀ a h, Finite (Range.SuccIterator (α := α) 1  (· ≤ a) h) Id] :
---     ForIn' m (PRange ⟨.unbounded, .closed⟩ α) α inferInstance where
---   forIn' r init f :=
---     ForIn'.forIn' (HasDownwardUnboundedRanges.min,,r.upper) init
---       fun out h acc => f out (by exact h.2) acc
+    refine ForIn'.forIn' (α := α) r.iterInternal init (fun a ha acc => f a ?_ acc)
+    simp only [Membership.mem] at ha
+    rwa [RangeIterator.isPlausibleIndirectOutput_iff] at ha
 
 end Iterator
 
-theorem Range.mem.upper [LE α] {i : α} {r : PRange ⟨.unbounded, .closed⟩ α} (h : i ∈ r) : i ≤ r.upper :=
-  h
+theorem Range.mem.upper [LE α] [DecidableLE α] {i : α} {r : PRange ⟨.unbounded, .closed⟩ α} (h : i ∈ r) : i ≤ r.upper :=
+  h.2
 
 -- theorem Range.mem.lower [LE α] {i : α} {r : PRange ⟨.unbounded, .closed⟩ α} (h : i ∈ r) : r.lower ≤ i := h.1
 
