src/Init/Data/Range/New/Classes.lean
@@ -2,19 +2,26 @@ module
 
 prelude
 import Init.Core
+import Init.Classical
 import Init.Data.Nat.Basic
-import Init.Data.Option.Basic
+import Init.Data.Option.Lemmas
 import Init.NotationExtra
 
 class UpwardEnumerable (α : Type u) where
   succ? : α → Option α
   succMany? (n : Nat) (a : α) : Option α := Nat.repeat (· >>= succ?) n (some a)
 
+@[expose]
 def UpwardEnumerable.le {α : Type u} [UpwardEnumerable α] (a b : α) : Prop :=
   ∃ n, UpwardEnumerable.succMany? n a = some b
 
+@[expose]
 def UpwardEnumerable.lt {α : Type u} [UpwardEnumerable α] (a b : α) : Prop :=
   ∃ n, UpwardEnumerable.succMany? (n + 1) a = some b
+
+theorem UpwardEnumerable.le_of_lt {α : Type u} [UpwardEnumerable α] {a b : α}
+    (h : UpwardEnumerable.lt a b) : UpwardEnumerable.le a b :=
+  ⟨h.choose + 1, h.choose_spec⟩
 
 -- Should we call it `OrderBot?` in analogy to Mathlib? Might be less clear to programmers.
 class Least? (α : Type u) extends UpwardEnumerable α where
@@ -29,6 +36,42 @@ class LawfulUpwardEnumerable (α : Type u) [UpwardEnumerable α] where
   succMany?_zero (a : α) : UpwardEnumerable.succMany? 0 a = some a
   succMany?_succ (n : Nat) (a : α) :
     UpwardEnumerable.succMany? (n + 1) a = (UpwardEnumerable.succMany? n a).bind UpwardEnumerable.succ?
+
+theorem UpwardEnumerable.succMany?_add [UpwardEnumerable α] [LawfulUpwardEnumerable α]
+    (m n : Nat) (a : α) :
+    UpwardEnumerable.succMany? (m + n) a = (UpwardEnumerable.succMany? m a).bind (UpwardEnumerable.succMany? n ·) := by
+  induction n
+  case zero => simp [LawfulUpwardEnumerable.succMany?_zero]
+  case succ n ih=>
+    rw [← Nat.add_assoc, LawfulUpwardEnumerable.succMany?_succ, ih, Option.bind_assoc]
+    simp only [LawfulUpwardEnumerable.succMany?_succ]
+
+theorem LawfulUpwardEnumerable.succMany?_succ_eq_succ_bind_succMany
+    [UpwardEnumerable α] [LawfulUpwardEnumerable α]
+    (n : Nat) (a : α) :
+    UpwardEnumerable.succMany? (n + 1) a = (UpwardEnumerable.succ? a).bind (UpwardEnumerable.succMany? n ·) := by
+  rw [Nat.add_comm]
+  simp [UpwardEnumerable.succMany?_add, LawfulUpwardEnumerable.succMany?_succ,
+    LawfulUpwardEnumerable.succMany?_zero]
+
+theorem UpwardEnumerable.le_refl {α : Type u} [UpwardEnumerable α] [LawfulUpwardEnumerable α]
+    (a : α) : UpwardEnumerable.le a a :=
+  ⟨0, LawfulUpwardEnumerable.succMany?_zero a⟩
+
+theorem UpwardEnumerable.le_trans {α : Type u} [UpwardEnumerable α] [LawfulUpwardEnumerable α]
+    {a b c : α} (hab : UpwardEnumerable.le a b) (hbc : UpwardEnumerable.le b c) :
+    UpwardEnumerable.le a c := by
+  refine ⟨hab.choose + hbc.choose, ?_⟩
+  simp [succMany?_add, hab.choose_spec, hbc.choose_spec]
+
+theorem UpwardEnumerable.not_gt_of_le {α : Type u} [UpwardEnumerable α] [LawfulUpwardEnumerable α]
+    {a b : α} :
+    UpwardEnumerable.le a b → ¬ UpwardEnumerable.lt b a := by
+  rintro ⟨n, hle⟩ ⟨m, hgt⟩
+  have : UpwardEnumerable.lt a a := by
+    refine ⟨n + m, ?_⟩
+    rw [Nat.add_assoc, UpwardEnumerable.succMany?_add, hle, Option.bind_some, hgt]
+  exact LawfulUpwardEnumerable.ne_of_lt _ _ this rfl
 
 class LawfulUpwardEnumerableLE (α : Type u) [UpwardEnumerable α] [LE α] where
   le_iff (a b : α) : a ≤ b ↔ UpwardEnumerable.le a b
@@ -46,23 +89,3 @@ class LawfulUpwardEnumerableLeast? (α : Type u) [UpwardEnumerable α] [Least? �
 --   mem_iff (a : α) (r : γ) :
 --     a ∈ r ↔ ∃ init, UpwardEnumerableMembership.init r = some init ∧ UpwardEnumerable.le init a ∧
 --       UpwardEnumerableMembership.Predicate r a
-
-instance : UpwardEnumerable Nat where
-  succ? n := some (n + 1)
-  succMany? k n := some (n + k)
-
-instance : Least? Nat where
-  least? := some 0
-
-instance : LawfulUpwardEnumerableLE Nat where
-  le_iff a b := sorry
-
-instance : LawfulUpwardEnumerableLT Nat where
-  lt_iff a b := sorry
-
-instance : LawfulUpwardEnumerable Nat where
-  succMany?_zero := by simp [UpwardEnumerable.succMany?]
-  succMany?_succ := by simp [UpwardEnumerable.succMany?, UpwardEnumerable.succ?, Bind.bind, Nat.add_assoc]
-  ne_of_lt a b hlt := by
-    rw [← LawfulUpwardEnumerableLT.lt_iff] at hlt
-    exact Nat.ne_of_lt hlt
