src/Init/Data/Range/New/Nat.lean
@@ -1,0 +1,172 @@
+prelude
+import Init.Data.Range.New.Iteration
+
+instance : UpwardEnumerable Nat where
+  succ? n := some (n + 1)
+  succMany? k n := some (n + k)
+
+instance : Least? Nat where
+  least? := some 0
+
+instance : LawfulUpwardEnumerableLE Nat where
+  le_iff a b := by
+    constructor
+    · intro h
+      exact ⟨b - a, by simp [UpwardEnumerable.succMany?, Nat.add_sub_cancel' h]⟩
+    · rintro ⟨n, hn⟩
+      simp only [UpwardEnumerable.succMany?, Option.some.injEq] at hn
+      rw [← hn]
+      exact Nat.le_add_right _ _
+
+instance : LawfulUpwardEnumerableLT Nat where
+  lt_iff a b := by
+    constructor
+    · intro h
+      refine ⟨b - a - 1, ?_⟩
+      simp [UpwardEnumerable.succMany?]
+      rw [Nat.sub_add_cancel, Nat.add_sub_cancel']
+      · exact Nat.le_of_lt h
+      · rwa [Nat.lt_iff_add_one_le, ← Nat.le_sub_iff_add_le'] at h
+        exact Nat.le_trans (Nat.le_succ _) h
+    · rintro ⟨n, hn⟩
+      simp only [UpwardEnumerable.succMany?, Option.some.injEq] at hn
+      rw [← hn]
+      apply Nat.lt_add_of_pos_right
+      apply Nat.zero_lt_succ
+
+instance : LawfulUpwardEnumerable Nat where
+  succMany?_zero := by simp [UpwardEnumerable.succMany?]
+  succMany?_succ := by simp [UpwardEnumerable.succMany?, UpwardEnumerable.succ?, Bind.bind, Nat.add_assoc]
+  ne_of_lt a b hlt := by
+    rw [← LawfulUpwardEnumerableLT.lt_iff] at hlt
+    exact Nat.ne_of_lt hlt
+
+instance : UpwardEnumerableRange ⟨.closed, .closed⟩ Nat where
+  init lowerBound := some lowerBound
+
+instance : LawfulUpwardEnumerableRange ⟨.closed, .closed⟩ Nat where
+  satisfiesUpperBound_of_le u a b hub hab := by
+    rw [← LawfulUpwardEnumerableLE.le_iff] at hab
+    exact Nat.le_trans hab hub
+  satisfiesLowerBound_iff a l := by
+    simp [← LawfulUpwardEnumerableLE.le_iff, UpwardEnumerableRange.init,
+      HasRange.SatisfiesLowerBound]
+
+instance : LawfulUpwardEnumerableRange ⟨.open, .closed⟩ Nat where
+  satisfiesUpperBound_of_le u a b hub hab := by
+    rw [← LawfulUpwardEnumerableLE.le_iff] at hab
+    exact Nat.le_trans hab hub
+  satisfiesLowerBound_iff a l := by
+    simp [← LawfulUpwardEnumerableLE.le_iff, UpwardEnumerableRange.init,
+      HasRange.SatisfiesLowerBound, UpwardEnumerable.succ?, Nat.lt_iff_add_one_le]
+
+instance : LawfulUpwardEnumerableRange ⟨.unbounded, .closed⟩ Nat where
+  satisfiesUpperBound_of_le u a b hub hab := by
+    rw [← LawfulUpwardEnumerableLE.le_iff] at hab
+    exact Nat.le_trans hab hub
+  satisfiesLowerBound_iff a l := by
+    simp [← LawfulUpwardEnumerableLE.le_iff, UpwardEnumerableRange.init,
+      HasRange.SatisfiesLowerBound, Nat.lt_iff_add_one_le, Least?.least?]
+
+instance : LawfulUpwardEnumerableRange ⟨.closed, .open⟩ Nat where
+  satisfiesUpperBound_of_le u a b hub hab := by
+    rw [← LawfulUpwardEnumerableLE.le_iff] at hab
+    exact Nat.lt_of_le_of_lt hab hub
+  satisfiesLowerBound_iff a l := by
+    simp [← LawfulUpwardEnumerableLE.le_iff, UpwardEnumerableRange.init,
+      HasRange.SatisfiesLowerBound]
+
+instance : LawfulUpwardEnumerableRange ⟨.open, .open⟩ Nat where
+  satisfiesUpperBound_of_le u a b hub hab := by
+    rw [← LawfulUpwardEnumerableLE.le_iff] at hab
+    exact Nat.lt_of_le_of_lt hab hub
+  satisfiesLowerBound_iff a l := by
+    simp [← LawfulUpwardEnumerableLE.le_iff, UpwardEnumerableRange.init,
+      HasRange.SatisfiesLowerBound, UpwardEnumerable.succ?, Nat.lt_iff_add_one_le]
+
+instance : LawfulUpwardEnumerableRange ⟨.unbounded, .open⟩ Nat where
+  satisfiesUpperBound_of_le u a b hub hab := by
+    rw [← LawfulUpwardEnumerableLE.le_iff] at hab
+    exact Nat.lt_of_le_of_lt hab hub
+  satisfiesLowerBound_iff a l := by
+    simp [← LawfulUpwardEnumerableLE.le_iff, UpwardEnumerableRange.init,
+      HasRange.SatisfiesLowerBound, Nat.lt_iff_add_one_le, Least?.least?]
+
+instance : LawfulUpwardEnumerableRange ⟨.closed, .unbounded⟩ Nat where
+  satisfiesUpperBound_of_le u a b hub hab := .intro
+  satisfiesLowerBound_iff a l := by
+    simp [← LawfulUpwardEnumerableLE.le_iff, UpwardEnumerableRange.init,
+      HasRange.SatisfiesLowerBound]
+
+instance : LawfulUpwardEnumerableRange ⟨.open, .unbounded⟩ Nat where
+  satisfiesUpperBound_of_le u a b hub hab := .intro
+  satisfiesLowerBound_iff a l := by
+    simp [← LawfulUpwardEnumerableLE.le_iff, UpwardEnumerableRange.init,
+      HasRange.SatisfiesLowerBound, UpwardEnumerable.succ?, Nat.lt_iff_add_one_le]
+
+instance : LawfulUpwardEnumerableRange ⟨.unbounded, .unbounded⟩ Nat where
+  satisfiesUpperBound_of_le u a b hub hab := .intro
+  satisfiesLowerBound_iff a l := by
+    simp [← LawfulUpwardEnumerableLE.le_iff, UpwardEnumerableRange.init,
+      HasRange.SatisfiesLowerBound, Nat.lt_iff_add_one_le, Least?.least?]
+
+private def rangeRev (k : Nat) :=
+  match k with
+  | 0 => []
+  | k + 1 => k :: rangeRev k
+
+private theorem mem_rangeRev {k l : Nat} (h : l < k) : l ∈ rangeRev k := by
+  induction k
+  case zero => cases h
+  case succ k ih =>
+    rw [rangeRev]
+    by_cases hl : l = k
+    · simp [hl]
+    · have : l < k := by
+        apply Nat.lt_of_le_of_ne
+        · exact Nat.le_of_lt_succ h
+        · exact hl
+      apply List.mem_cons_of_mem
+      exact ih this
+
+instance : FinitelyEnumerableRange ⟨.closed, .closed⟩ Nat where
+  enumeration upperBound := rangeRev (upperBound + 1)
+  mem_enumeration_of_satisfiesUpperBound upperBound a h := by
+    simp only [HasRange.SatisfiesUpperBound] at h
+    apply mem_rangeRev
+    exact Nat.lt_succ_of_le h
+
+instance : FinitelyEnumerableRange ⟨.open, .closed⟩ Nat where
+  enumeration upperBound := rangeRev (upperBound + 1)
+  mem_enumeration_of_satisfiesUpperBound upperBound a h := by
+    simp only [HasRange.SatisfiesUpperBound] at h
+    apply mem_rangeRev
+    exact Nat.lt_succ_of_le h
+
+instance : FinitelyEnumerableRange ⟨.unbounded, .closed⟩ Nat where
+  enumeration upperBound := rangeRev (upperBound + 1)
+  mem_enumeration_of_satisfiesUpperBound upperBound a h := by
+    simp only [HasRange.SatisfiesUpperBound] at h
+    apply mem_rangeRev
+    exact Nat.lt_succ_of_le h
+
+instance : FinitelyEnumerableRange ⟨.closed, .open⟩ Nat where
+  enumeration upperBound := rangeRev (upperBound + 1)
+  mem_enumeration_of_satisfiesUpperBound upperBound a h := by
+    simp only [HasRange.SatisfiesUpperBound] at h
+    apply mem_rangeRev
+    exact Nat.lt_succ_of_lt h
+
+instance : FinitelyEnumerableRange ⟨.open, .open⟩ Nat where
+  enumeration upperBound := rangeRev (upperBound + 1)
+  mem_enumeration_of_satisfiesUpperBound upperBound a h := by
+    simp only [HasRange.SatisfiesUpperBound] at h
+    apply mem_rangeRev
+    exact Nat.lt_succ_of_lt h
+
+instance : FinitelyEnumerableRange ⟨.unbounded, .open⟩ Nat where
+  enumeration upperBound := rangeRev (upperBound + 1)
+  mem_enumeration_of_satisfiesUpperBound upperBound a h := by
+    simp only [HasRange.SatisfiesUpperBound] at h
+    apply mem_rangeRev
+    exact Nat.lt_succ_of_lt h
