src/Init/Data/Range/New/RangeIterator.lean
@@ -114,9 +114,6 @@ instance RepeatIterator.instIteratorCollectPartial [UpwardEnumerable α] [HasRan
     {n : Type u → Type w} [Monad n] : IteratorCollectPartial (RangeIterator shape α) Id n :=
   .defaultImplementation
 
-instance RepeatIterator.instFinite [UpwardEnumerable α] [HasRange shape α] :
-    Finite (RangeIterator shape α) Id := sorry
-
 -- TODO: very specific performance optimizations if needed
 
 -- abbrev test : ForIn Id (Iter (α := RangeIterator α instSucc? p) α) α :=
@@ -221,5 +218,83 @@ theorem RangeIterator.isPlausibleSuccessorOf_iff
         UpwardEnumerable.succ? a = it'.internalState.next ∧
         it'.internalState.upperBound = it.internalState.upperBound := by
   simp [Iter.IsPlausibleSuccessorOf, Monadic.isPlausibleSuccessorOf_iff, Iter.toIterM]
+
+theorem RangeIterator.isSome_next_of_isPlausibleIndirectOutput
+    [UpwardEnumerable α] [HasRange shape α]
+    {it : Iter (α := RangeIterator shape α) α} {out : α}
+    (h : it.IsPlausibleIndirectOutput out) :
+    it.internalState.next.isSome := by
+  cases h
+  case direct h =>
+    rw [isPlausibleOutput_iff] at h
+    simp [h]
+  case indirect h _ =>
+    rw [isPlausibleSuccessorOf_iff] at h
+    obtain ⟨a, ha, _⟩ := h
+    simp [ha]
+
+private def List.Sublist.filter_mono {l : List α} {P Q : α → Bool} (h : ∀ a, P a → Q a) :
+    List.Sublist (l.filter P) (l.filter Q) := by
+  apply List.Sublist.trans (l₂ := (l.filter Q).filter P)
+  · simp [Bool.and_eq_left_iff_imp.mpr (h _)]
+  · apply List.filter_sublist
+
+private def List.length_filter_strict_mono {l : List α} {P Q : α → Bool} {a : α}
+    (h : ∀ a, P a → Q a) (ha : a ∈ l) (hPa : ¬ P a) (hQa : Q a) :
+    (l.filter P).length < (l.filter Q).length := by
+  have hsl : List.Sublist (l.filter P) (l.filter Q) := by
+    apply List.Sublist.filter_mono
+    exact h
+  apply Nat.lt_of_le_of_ne
+  · apply List.Sublist.length_le
+    exact hsl
+  · intro h
+    apply hPa
+    have heq := List.Sublist.eq_of_length hsl h
+    have : a ∈ List.filter Q l := List.mem_filter.mpr ⟨ha, hQa⟩
+    rw [← heq, List.mem_filter] at this
+    exact this.2
+
+def RangeIterator.instFinitenessRelation [UpwardEnumerable α] [HasRange shape α]
+    [UpwardEnumerableRange shape α] [LawfulUpwardEnumerableRange shape α]
+    [LawfulUpwardEnumerable α] [FinitelyEnumerableRange shape α] :
+    FinitenessRelation (RangeIterator shape α) Id where
+  rel :=
+    open Classical in
+    InvImage WellFoundedRelation.rel
+      (fun it => FinitelyEnumerableRange.enumeration it.internalState.upperBound
+        |>.filter (∃ a, it.internalState.next = some a ∧ UpwardEnumerable.le a ·)
+        |>.length)
+  wf := InvImage.wf _ WellFoundedRelation.wf
+  subrelation {it it'} h := by
+    simp_wf
+    rw [Monadic.isPlausibleSuccessorOf_iff] at h
+    obtain ⟨a, hn, hu, hn', hu'⟩ := h
+    rw [hu']
+    apply List.length_filter_strict_mono (a := a)
+    · intro u h
+      simp only [decide_eq_true_eq] at ⊢ h
+      obtain ⟨a', ha', hle⟩ := h
+      refine ⟨a, hn, UpwardEnumerable.le_trans ?_ hle⟩
+      refine ⟨1, ?_⟩
+      rw [ha'] at hn'
+      rw [LawfulUpwardEnumerable.succMany?_succ, LawfulUpwardEnumerable.succMany?_zero,
+        Option.bind_some, hn']
+    · exact FinitelyEnumerableRange.mem_enumeration_of_satisfiesUpperBound _ _ hu
+    · intro h
+      simp only [decide_eq_true_eq] at h
+      obtain ⟨x, hx, h⟩ := h
+      rw [hx] at hn'
+      have hlt : UpwardEnumerable.lt a x :=
+        ⟨0, by simp [LawfulUpwardEnumerable.succMany?_succ, LawfulUpwardEnumerable.succMany?_zero, hn']⟩
+      exact UpwardEnumerable.not_gt_of_le h hlt
+    · simp only [decide_eq_true_eq]
+      exact ⟨a, hn, UpwardEnumerable.le_refl _⟩
+
+instance RangeIterator.instFinite [UpwardEnumerable α] [HasRange shape α]
+    [UpwardEnumerableRange shape α] [LawfulUpwardEnumerableRange shape α]
+    [LawfulUpwardEnumerable α] [FinitelyEnumerableRange shape α] :
+    Finite (RangeIterator shape α) Id :=
+  .of_finitenessRelation instFinitenessRelation
 
 end Std.Iterators.Types
